lean/LoVe/LoVe05_FunctionalProgramming_HomeworkSheet.lean
@@ -33,16 +33,19 @@ numeric weight, a left subtree, and a right subtree.
 tree over some type variable `α` and that returns the weight component of the
 root node of the tree: -/
 
-def weight {α : Type} : HTree α → ℕ :=
-  sorry
+def weight {α : Type} : HTree α → ℕ
+  | HTree.leaf w _ => w
+  | HTree.inner w l r => w + weight l + weight r
 
 /- 1.2 (1 point). Define a polymorphic Lean function called `unite` that takes
 two trees `l, r : HTree α` and that returns a new tree such that (1) its left
 child is `l`; (2) its right child is `r`; and (3) its weight is the sum of the
 weights of `l` and `r`. -/
 
-def unite {α : Type} : HTree α → HTree α → HTree α :=
-  sorry
+def unite {α : Type} : HTree α → HTree α → HTree α
+  | t₁, t₂ => 
+    let s := weight t₁ + weight t₂
+    HTree.inner s t₁ t₂
 
 /- 1.3 (2 points). Consider the following `insort` function, which inserts a
 tree `u` in a list of trees that is sorted by increasing weight and which
@@ -56,8 +59,14 @@ def insort {α : Type} (u : HTree α) : List (HTree α) → List (HTree α)
 /- Prove that `insort`ing a tree into a list cannot yield the empty list: -/
 
 theorem insort_Neq_nil {α : Type} (t : HTree α) :
-  ∀ts : List (HTree α), insort t ts ≠ [] :=
-  sorry
+  ∀ts : List (HTree α), insort t ts ≠ [] := by
+  intro ts
+  cases ts with
+  | nil => simp [insort]
+  | cons x xs => 
+    cases Classical.em (weight t ≤ weight x)
+    . simp [insort, h]
+    . simp [insort, h]
 
 /- 1.4 (2 points). Prove the same property as above again, this time as a
 "paper" proof. Follow the guidelines given in question 1.4 of the exercise. -/
@@ -93,15 +102,27 @@ Hints:
 #check add_mul
 
 theorem sumUpToOfFun_eq :
-  ∀m : ℕ, 2 * sumUpToOfFun (fun i ↦ i) m = m * (m + 1) :=
-  sorry
+  ∀m : ℕ, 2 * sumUpToOfFun (fun i ↦ i) m = m * (m + 1) := by
+  intro n
+  induction n with
+  | zero => simp [sumUpToOfFun]
+  | succ n' => 
+    simp [sumUpToOfFun]
+    rw [mul_add, n_ih]
+    linarith
 
 /- 2.2 (2 points). Prove the following property of `sumUpToOfFun`. -/
 
 theorem sumUpToOfFun_mul (f g : ℕ → ℕ) :
   ∀n : ℕ, sumUpToOfFun (fun i ↦ f i + g i) n =
-    sumUpToOfFun f n + sumUpToOfFun g n :=
-  sorry
+    sumUpToOfFun f n + sumUpToOfFun g n := by
+  intro n
+  induction n with
+  | zero => simp [sumUpToOfFun]
+  | succ n' =>
+    simp [sumUpToOfFun]
+    rw [n_ih]
+    linarith
 
 /- 2.3 (2 bonus points). Prove `sumUpToOfFun_mul` again as a "paper" proof.
 Follow the guidelines given in question 1.4 of the exercise. -/
