lean/LoVe/LoVe06_InductivePredicates_ExerciseSheet.lean
@@ -32,21 +32,31 @@ Hint: `cases` or `induction` is useful to reason about hypotheses of the form
 `Even …`. -/
 
 @[simp] theorem Odd_1 :
-  Odd 1 :=
-  sorry
+  Odd 1 := by
+  intro he
+  cases he
 
 /- 1.2. Prove that 3 and 5 are odd. -/
 
--- enter your answer here
+theorem Odd_3 : Odd 3 := by
+  intro he
+  cases he
+  cases a
+
+theorem Odd_5 : Odd 5 := by
+  intro he
+  cases he
+  cases a
+  cases a_1
 
 /- 1.3. Complete the following proof by structural induction. -/
+
+#check Even.add_two
 
 theorem Even_two_times :
   ∀m : ℕ, Even (2 * m)
   | 0     => Even.zero
-  | m + 1 =>
-    sorry
-
+  | m + 1 => Even.add_two (2*m) (Even_two_times m)
 
 /- ## Question 2: Tennis Games
 
@@ -58,29 +68,33 @@ Recall the inductive type of tennis scores from the demo: -/
 ahead of the receiver and that returns `False` otherwise. -/
 
 inductive ServAhead : Score → Prop
-  -- enter the missing cases here
+  | vs m n    : m > n → ServAhead (Score.vs m n)
+  | adv_serv  : ServAhead Score.advServ
+  | game_serv : ServAhead Score.gameServ
 
 /- 2.2. Validate your predicate definition by proving the following theorems. -/
 
 theorem ServAhead_vs {m n : ℕ} (hgt : m > n) :
   ServAhead (Score.vs m n) :=
-  sorry
+  ServAhead.vs m n hgt
 
 theorem ServAhead_advServ :
   ServAhead Score.advServ :=
-  sorry
+  ServAhead.adv_serv
 
 theorem not_ServAhead_advRecv :
-  ¬ ServAhead Score.advRecv :=
-  sorry
+  ¬ ServAhead Score.advRecv := by
+  intro h
+  cases h
 
 theorem ServAhead_gameServ :
   ServAhead Score.gameServ :=
-  sorry
+  ServAhead.game_serv
 
 theorem not_ServAhead_gameRecv :
-  ¬ ServAhead Score.gameRecv :=
-  sorry
+  ¬ ServAhead Score.gameRecv := by
+  intro h
+  cases h
 
 /- 2.3. Compare the above theorem statements with your definition. What do you
 observe? -/
@@ -97,24 +111,46 @@ theorems (e.g., `IsFull_mirror`, `mirror_mirror`). -/
 #check mirror_mirror
 
 theorem mirror_IsFull {α : Type} :
-  ∀t : Tree α, IsFull (mirror t) → IsFull t :=
-  sorry
+  ∀t : Tree α, IsFull (mirror t) → IsFull t := by
+  intro t hf
+  have hm : IsFull (mirror (mirror t)) := IsFull_mirror _ hf
+  rw [←mirror_mirror t]
+  exact hm
 
 /- 3.2. Define a `map` function on binary trees, similar to `List.map`. -/
 
-def Tree.map {α β : Type} (f : α → β) : Tree α → Tree β :=
-  sorry
+#print Tree
+
+def Tree.map {α β : Type} (f : α → β) : Tree α → Tree β
+  | Tree.nil => Tree.nil
+  | Tree.node a l r => Tree.node (f a) (map f l) (map f r)
 
 /- 3.3. Prove the following theorem by case distinction. -/
 
 theorem Tree.map_eq_empty_iff {α β : Type} (f : α → β) :
-  ∀t : Tree α, Tree.map f t = Tree.nil ↔ t = Tree.nil :=
-  sorry
+  ∀t : Tree α, Tree.map f t = Tree.nil ↔ t = Tree.nil := by
+  intro t
+  cases t
+  . simp [Tree.map]
+  . simp [Tree.map]
 
 /- 3.4 (**optional**). Prove the following theorem by rule induction. -/
 
 theorem map_mirror {α β : Type} (f : α → β) :
-  ∀t : Tree α, IsFull t → IsFull (Tree.map f t) :=
-  sorry
-
+  ∀t : Tree α, IsFull t → IsFull (Tree.map f t) := by
+  intro t ht
+  induction ht with
+  | nil => 
+    simp [Tree.map]
+    exact IsFull.nil
+  | node a l r hl hr hiff hl_ih hr_ih =>
+    simp [Tree.map]
+    apply IsFull.node
+    { exact hl_ih }
+    { exact hr_ih }
+    { 
+      simp [Tree.map_eq_empty_iff]
+      exact hiff
+    }
+  
 end LoVe
