lean/LoVe/LoVe11_DenotationalSemantics_ExerciseSheet.lean
@@ -21,16 +21,28 @@ namespace LoVe
 
 theorem Monotone_restrict {α β : Type} [PartialOrder α] (f : α → Set (β × β))
     (p : β → Prop) (hf : Monotone f) :
-  Monotone (fun a ↦ f a ⇃ p) :=
-  sorry
+  Monotone (fun a ↦ f a ⇃ p) := by
+  intro a₁ a₂ ha
+  simp
+  simp [restrict]
+  intro a b hab hpa
+  apply And.intro
+  . exact hf a₁ a₂ ha hab
+  . exact hpa
 
 /- 1.2. Prove its cousin. -/
 
 theorem Monotone_comp {α β : Type} [PartialOrder α] (f g : α → Set (β × β))
     (hf : Monotone f) (hg : Monotone g) :
-  Monotone (fun a ↦ f a ◯ g a) :=
-  sorry
-
+  Monotone (fun a ↦ f a ◯ g a) := by
+  intro a₁ a₂ ha
+  simp
+  simp [comp]
+  intro a b c hac hcb
+  apply Exists.intro c
+  apply And.intro
+  . exact hf a₁ a₂ ha hac
+  . exact hg a₁ a₂ ha hcb
 
 /- ## Question 2: Regular Expressions
 
@@ -84,13 +96,22 @@ Hint: Exploit the correspondence with the WHILE language. -/
 def rel_of_Regex {α : Type} : Regex (Set (α × α)) → Set (α × α)
   | Regex.nothing      => ∅
   | Regex.empty        => Id
-  -- enter the missing cases here
+  | Regex.atom a       => a
+  | Regex.concat r₁ r₂ => rel_of_Regex r₁ ◯ rel_of_Regex r₂
+  | Regex.alt r₁ r₂    => rel_of_Regex r₁ ∪ rel_of_Regex r₂
+  | Regex.star r       => lfp (fun S ↦ (rel_of_Regex r ◯ S) ∪ Id)
 
 /- 2.2. Prove the following recursive equation about your definition. -/
 
 theorem rel_of_Regex_Star {α : Type} (r : Regex (Set (α × α))) :
   rel_of_Regex (Regex.star r) =
-  rel_of_Regex (Regex.alt (Regex.concat r (Regex.star r)) Regex.empty) :=
-  sorry
+  rel_of_Regex (Regex.alt (Regex.concat r (Regex.star r)) Regex.empty) := by
+  simp [rel_of_Regex]
+  apply lfp_eq
+  apply Monotone_union
+  . apply Monotone_comp
+    . apply Monotone_const
+    . apply Monotone_id
+  . apply Monotone_const
 
 end LoVe
