lean/LoVe/LoVe12_LogicalFoundationsOfMathematics_HomeworkSheet.lean
@@ -34,7 +34,7 @@ predicate introduced in the lecture 5 demo. -/
 #print Even
 
 def Eveℕ : Type :=
-  sorry
+  {t : ℕ // Even t}
 
 /- 1.2 (1 point). Prove the following theorem about the `Even` predicate. You will
 need it to answer question 1.3.
@@ -42,36 +42,51 @@ need it to answer question 1.3.
 Hint: The theorems `add_assoc` and `add_comm` might be useful. -/
 
 theorem Even.add {m n : ℕ} (hm : Even m) (hn : Even n) :
-  Even (m + n) :=
-  sorry
+  Even (m + n) := by
+  induction hm
+  . simp
+    exact hn
+  . simp [add_comm k, add_assoc]
+    rw [add_comm]
+    apply Even.add_two
+    rw [add_comm]
+    exact a_ih
 
 /- 1.3 (2 points). Define zero and addition of even numbers by filling in the
 `sorry` placeholders. -/
 
 def Eveℕ.zero : Eveℕ :=
-  sorry
+  Subtype.mk 0 Even.zero
 
 def Eveℕ.add (m n : Eveℕ) : Eveℕ :=
-  sorry
+  Subtype.mk (Subtype.val m + Subtype.val n) (Even.add (Subtype.property m) (Subtype.property n))
 
 /- 1.4 (4 points). Prove that addition of even numbers is commutative and
 associative, and has 0 as an identity element. -/
 
 theorem Eveℕ.add_comm (m n : Eveℕ) :
-  Eveℕ.add m n = Eveℕ.add n m :=
-  sorry
+  Eveℕ.add m n = Eveℕ.add n m := by
+  apply Subtype.eq
+  simp [Eveℕ.add]
+  linarith
 
 theorem Eveℕ.add_assoc (l m n : Eveℕ) :
-  Eveℕ.add (Eveℕ.add l m) n = Eveℕ.add l (Eveℕ.add m n) :=
-  sorry
+  Eveℕ.add (Eveℕ.add l m) n = Eveℕ.add l (Eveℕ.add m n) := by
+  apply Subtype.eq
+  simp [Eveℕ.add]
+  linarith
 
 theorem Eveℕ.add_iden_left (n : Eveℕ) :
-  Eveℕ.add Eveℕ.zero n = n :=
-  sorry
+  Eveℕ.add Eveℕ.zero n = n := by
+  apply Subtype.eq
+  simp [Eveℕ.add]
+  rfl
 
 theorem Eveℕ.add_iden_right (n : Eveℕ) :
-  Eveℕ.add n Eveℕ.zero = n :=
-  sorry
+  Eveℕ.add n Eveℕ.zero = n := by
+  apply Subtype.eq
+  simp [Eveℕ.add]
+  rfl
 
 
 /- ## Question 2 (2 points + 2 bonus points): Hilbert Choice
@@ -85,11 +100,25 @@ Hints:
 
 * The theorem `le_of_not_gt` might be useful. -/
 
+#check le_of_not_gt
+
 theorem exists_minimal_arg_helper (f : ℕ → ℕ) :
   ∀x m, f m = x → ∃n, ∀i, f n ≤ f i
 | x, m, eq =>
   by
-    sorry, sorry
+    have em := Classical.em (∃n, f n < x)
+    cases em
+    . cases h
+      apply exists_minimal_arg_helper f (f w) w
+      rfl
+    . apply Exists.intro m
+      intro i
+      rw [eq]
+      apply le_of_not_gt
+      intro hx
+      apply h
+      apply Exists.intro i
+      exact hx
 
 /- Now this interesting theorem falls off: -/
 
@@ -102,13 +131,13 @@ define the following function, which returns the (or an) index of the minimal
 element in `f`'s image. -/
 
 noncomputable def minimal_arg (f : ℕ → ℕ) : ℕ :=
-  sorry
+  Classical.choose (exists_minimal_arg f)
 
 /- 2.3 (1 point). Prove the following characteristic theorem about your
 definition. -/
 
 theorem minimal_arg_spec (f : ℕ → ℕ) :
   ∀i : ℕ, f (minimal_arg f) ≤ f i :=
-  sorry
+  Classical.choose_spec (exists_minimal_arg f)
 
 end LoVe
