lean/LoVe/LoVe03_BackwardProofs_ExerciseSheet.lean
@@ -25,36 +25,44 @@ Hint: Some strategies for carrying out such proofs are described at the end of
 Section 3.3 in the Hitchhiker's Guide. -/
 
 theorem I (a : Prop) :
-  a → a :=
-  sorry
+  a → a := by
+  intro ha
+  apply ha
 
 theorem K (a b : Prop) :
-  a → b → b :=
-  sorry
+  a → b → b := by
+  intro ha hb
+  apply hb
 
 theorem C (a b c : Prop) :
-  (a → b → c) → b → a → c :=
-  sorry
+  (a → b → c) → b → a → c := by
+  intro f b a
+  apply f a b
 
 theorem proj_fst (a : Prop) :
-  a → a → a :=
-  sorry
+  a → a → a := by
+  intro ha ha'
+  apply ha
 
 /- Please give a different answer than for `proj_fst`: -/
 
 theorem proj_snd (a : Prop) :
-  a → a → a :=
-  sorry
+  a → a → a := by
+  intro ha ha'
+  apply ha'
 
 theorem some_nonsense (a b c : Prop) :
-  (a → b → c) → a → (a → c) → b → c :=
-  sorry
+  (a → b → c) → a → (a → c) → b → c := by
+  intro f a g b
+  apply g a
 
 /- 1.2. Prove the contraposition rule using basic tactics. -/
 
 theorem contrapositive (a b : Prop) :
-  (a → b) → ¬ b → ¬ a :=
-  sorry
+  (a → b) → ¬ b → ¬ a := by
+  intro f hnb ha
+  apply hnb
+  apply f ha
 
 /- 1.3. Prove the distributivity of `∀` over `∧` using basic tactics.
 
@@ -63,8 +71,19 @@ forward reasoning, like in the proof of `and_swap_braces` in the lecture, might
 be necessary. -/
 
 theorem forall_and {α : Type} (p q : α → Prop) :
-  (∀x, p x ∧ q x) ↔ (∀x, p x) ∧ (∀x, q x) :=
-  sorry
+  (∀x, p x ∧ q x) ↔ (∀x, p x) ∧ (∀x, q x) := by
+  apply Iff.intro
+  . intro h
+    apply And.intro
+    . intro x
+      exact And.left (h x)
+    . intro x
+      apply And.right (h x)
+  . intro h
+    intro x
+    apply And.intro
+    . apply (And.left h) x
+    . apply (And.right h) x
 
 
 /- ## Question 2: Natural Numbers
@@ -75,32 +94,49 @@ theorem forall_and {α : Type} (p q : α → Prop) :
 #check mul
 
 theorem mul_zero (n : ℕ) :
-  mul 0 n = 0 :=
-  sorry
+  mul 0 n = 0 := by
+  induction n with
+  | zero => rfl
+  | succ n => 
+    simp [mul]
+    rw [n_ih]
+    rfl
 
 #check add_succ
 theorem mul_succ (m n : ℕ) :
-  mul (Nat.succ m) n = add (mul m n) n :=
-  sorry
+  mul (Nat.succ m) n = add (mul m n) n := by
+  induction n with
+  | zero => rfl
+  | succ n => 
+    simp [mul, add_succ, n_ih]
+    nth_rw 3 [add_comm]
+    rw [add_succ]
+    ac_rfl
+
 
 /- 2.2. Prove commutativity and associativity of multiplication using the
 `induction` tactic. Choose the induction variable carefully. -/
 
 theorem mul_comm (m n : ℕ) :
-  mul m n = mul n m :=
-  sorry
+  mul m n = mul n m := by
+  induction m with
+  | zero => simp [mul, mul_zero]
+  | succ m => 
+    simp [mul, mul_succ, n_ih, add_comm]
 
 theorem mul_assoc (l m n : ℕ) :
-  mul (mul l m) n = mul l (mul m n) :=
-  sorry
+  mul (mul l m) n = mul l (mul m n) := by
+  induction n with
+  | zero => simp [mul, mul_zero]
+  | succ n =>
+    simp [mul, mul_succ, n_ih, mul_add]
 
 /- 2.3. Prove the symmetric variant of `mul_add` using `rw`. To apply
 commutativity at a specific position, instantiate the rule by passing some
 arguments (e.g., `mul_comm _ l`). -/
-
 theorem add_mul (l m n : ℕ) :
-  mul (add l m) n = add (mul n l) (mul n m) :=
-  sorry
+  mul (add l m) n = add (mul n l) (mul n m) := by
+  rw [mul_comm, mul_add]
 
 
 /- ## Question 3 (**optional**): Intuitionistic Logic
@@ -127,23 +163,52 @@ Hint: You will need `Or.elim` and `False.elim`. You can use
 `rw [ExcludedMiddle]` to unfold the definition of `ExcludedMiddle`,
 and similarly for `Peirce`. -/
 
+#check Or.elim
+
 theorem Peirce_of_EM :
-  ExcludedMiddle → Peirce :=
-  sorry
+  ExcludedMiddle → Peirce := by
+  rw [ExcludedMiddle, Peirce]
+  intro em a b f
+  apply Or.elim (em a)
+  . intro a'
+    apply a'
+  . intro na
+    apply f
+    intro a'
+    apply False.elim
+    apply na
+    apply a'
 
 /- 3.2 (**optional**). Prove the following implication using tactics. -/
 
 theorem DN_of_Peirce :
-  Peirce → DoubleNegation :=
-  sorry
+  Peirce → DoubleNegation := by
+  rw [Peirce, DoubleNegation]
+  intro h a nna
+  apply (h a False)
+  intro g
+  apply False.elim
+  apply nna
+  intro a'
+  apply g
+  apply a'
 
 /- We leave the remaining implication for the homework: -/
 
 namespace SorryTheorems
 
 theorem EM_of_DN :
-  DoubleNegation → ExcludedMiddle :=
-sorry
+  DoubleNegation → ExcludedMiddle := by
+  rw [ExcludedMiddle]
+  intro dn a
+  apply dn
+  intro h
+  apply h
+  right
+  intro a'
+  apply h
+  left
+  apply a'
 
 end SorryTheorems
 
