lean/LoVe/LoVe03_BackwardProofs_HomeworkSheet.lean
@@ -28,26 +28,40 @@ Hint: Some strategies for carrying out such proofs are described at the end of
 Section 3.3 in the Hitchhiker's Guide. -/
 
 theorem B (a b c : Prop) :
-  (a → b) → (c → a) → c → b :=
-  sorry
+  (a → b) → (c → a) → c → b := by
+  intro h₁ h₂ hc
+  apply h₁
+  apply h₂
+  apply hc
 
 theorem S (a b c : Prop) :
-  (a → b → c) → (a → b) → a → c :=
-  sorry
+  (a → b → c) → (a → b) → a → c := by
+  intro h₁ h₂ ha
+  apply (h₁ ha (h₂ ha))
 
 theorem more_nonsense (a b c d : Prop) :
-  ((a → b) → c → d) → c → b → d :=
-  sorry
+  ((a → b) → c → d) → c → b → d := by
+  intro h₁ hc hb
+  apply (h₁ (fun _ ↦ hb) hc)
 
 theorem even_more_nonsense (a b c : Prop) :
-  (a → b) → (a → c) → a → b → c :=
-  sorry
+  (a → b) → (a → c) → a → b → c := by
+  intro h₁ h₂ ha hb
+  apply h₂
+  apply ha
 
 /- 1.2 (1 point). Prove the following theorem using basic tactics. -/
 
 theorem weak_peirce (a b : Prop) :
-  ((((a → b) → a) → a) → b) → b :=
-  sorry
+  ((((a → b) → a) → a) → b) → b := by
+  intro p
+  apply p
+  intro q
+  apply q
+  intro a'
+  apply p
+  intro r
+  apply a'
 
 
 /- ## Question 2 (5 points): Logical Connectives
@@ -64,8 +78,17 @@ Hints:
   proof. -/
 
 theorem herman (a : Prop) :
-  ¬¬ (¬¬ a → a) :=
-  sorry
+  ¬¬ (¬¬ a → a) := by
+  rw [Not]
+  intro f
+  apply f
+  intro nna
+  apply False.elim
+  apply nna
+  intro a'
+  apply f
+  intro nna'
+  apply a'
 
 /- 2.2 (2 points). Prove the missing link in our chain of classical axiom
 implications.
@@ -89,8 +112,17 @@ Hints:
 #check ExcludedMiddle
 
 theorem EM_of_DN :
-  DoubleNegation → ExcludedMiddle :=
-  sorry
+  DoubleNegation → ExcludedMiddle := by
+  rw [ExcludedMiddle]
+  intro dn a
+  apply dn
+  intro h
+  apply h
+  right
+  intro a'
+  apply h
+  left
+  apply a'
 
 /- 2.3 (2 points). We have proved three of the six possible implications
 between `ExcludedMiddle`, `Peirce`, and `DoubleNegation`. State and prove the
@@ -100,7 +132,27 @@ three missing implications, exploiting the three theorems we already have. -/
 #check DN_of_Peirce
 #check EM_of_DN
 
--- enter your solution here
+theorem Peirce_of_DN :
+  DoubleNegation → Peirce := by
+  intro dn
+  apply Peirce_of_EM
+  apply EM_of_DN
+  apply dn
+
+theorem EM_of_Peirce :
+  Peirce → ExcludedMiddle := by
+  intro p
+  apply EM_of_DN
+  apply DN_of_Peirce
+  apply p
+
+theorem DN_of_EM :
+  ExcludedMiddle → DoubleNegation := by
+  intro em
+  apply DN_of_Peirce
+  apply Peirce_of_EM
+  apply em
+
 
 end BackwardProofs
 
