lean/LoVe/LoVe04_ForwardProofs_ExerciseSheet.lean
@@ -19,49 +19,85 @@ namespace LoVe
 
 theorem I (a : Prop) :
   a → a :=
-  sorry
+  assume ha : a
+  show a from ha
 
 theorem K (a b : Prop) :
   a → b → b :=
-  sorry
+  assume ha : a
+  assume hb : b
+  show b from hb
 
 theorem C (a b c : Prop) :
   (a → b → c) → b → a → c :=
-  sorry
+  assume habc : a → b → c
+  assume hb : b
+  assume ha : a
+  show c from habc ha hb
 
 theorem proj_fst (a : Prop) :
   a → a → a :=
-  sorry
+  assume ha₁ : a
+  assume ha₂ : a
+  show a from ha₁
 
 /- Please give a different answer than for `proj_fst`. -/
 
 theorem proj_snd (a : Prop) :
   a → a → a :=
-  sorry
+  assume ha₁ : a
+  assume ha₂ : a
+  show a from ha₂
 
 theorem some_nonsense (a b c : Prop) :
   (a → b → c) → a → (a → c) → b → c :=
-  sorry
+  assume habc : a → b → c
+  assume ha : a
+  assume hac : a → c
+  assume hb : b
+  show c from hac ha
 
 /- 1.2. Supply a structured proof of the contraposition rule. -/
 
 theorem contrapositive (a b : Prop) :
   (a → b) → ¬ b → ¬ a :=
-  sorry
+  assume hab : a → b
+  assume hnb : ¬ b
+  assume ha : a
+  show False from
+    hnb (hab ha)
 
 /- 1.3. Supply a structured proof of the distributivity of `∀` over `∧`. -/
 
 theorem forall_and {α : Type} (p q : α → Prop) :
   (∀x, p x ∧ q x) ↔ (∀x, p x) ∧ (∀x, q x) :=
-  sorry
+  Iff.intro
+    (assume hfa : ∀x, p x ∧ q x
+    have hpx : ∀x, p x :=
+      fix x : α
+      show p x from And.left (hfa x)
+    have hqx : ∀x, q x :=
+      fix x : α
+      show q x from And.right (hfa x)
+    show (∀x, p x) ∧ (∀x, q x) from And.intro hpx hqx)
+    (assume hlr : (∀x, p x) ∧ (∀x, q x)
+    fix x : α
+    have hpx := hlr.left x
+    have hqx := hlr.right x
+    show p x ∧ q x from
+      And.intro hpx hqx)
 
 /- 1.4 (**optional**). Supply a structured proof of the following property,
 which can be used to pull a `∀` quantifier past an `∃` quantifier. -/
 
 theorem forall_exists_of_exists_forall {α : Type} (p : α → α → Prop) :
   (∃x, ∀y, p x y) → (∀y, ∃x, p x y) :=
-  sorry
-
+  assume hef : ∃x, ∀y, p x y
+  fix y : α
+  Exists.elim hef 
+    (fix x : α
+     assume hpxy : ∀y, p x y
+     Exists.intro x (hpxy y))
 
 /- ## Question 2: Chain of Equalities
 
@@ -77,9 +113,23 @@ Hint: This is a difficult question. You might need the tactics `simp` and
 `ac_rfl` and some of the theorems `mul_add`, `add_mul`, `add_comm`, `add_assoc`,
 `mul_comm`, `mul_assoc`, , and `Nat.two_mul`. -/
 
+#check mul_add
+#check add_mul
+#check add_comm
+#check add_assoc
+#check mul_comm
+#check mul_assoc
+#check Nat.two_mul
+
 theorem binomial_square (a b : ℕ) :
   (a + b) * (a + b) = a * a + 2 * a * b + b * b :=
-  sorry
+  calc
+    (a + b) * (a + b) = a * (a + b) + b * (a + b) := by rw [add_mul]
+    _ = a * a + a * b + b * a + b * b := by simp [mul_add, add_assoc]
+    _ = a * a + a * b + a * b + b * b := by simp [mul_comm]
+    _ = a * a + (a * b + a * b) + b * b := by simp [add_assoc]
+    _ = a * a + (2 * (a * b)) + b * b := by rw [← Nat.two_mul]
+    _ = a * a + 2 * a * b + b * b := by simp [add_assoc, mul_assoc]
 
 /- 2.2 (**optional**). Prove the same argument again, this time as a structured
 proof, with `have` steps corresponding to the `calc` equations. Try to reuse as
@@ -100,7 +150,12 @@ axiom All.one_point_wrong {α : Type} (t : α) (P : α → Prop) :
 
 theorem All.proof_of_False :
   False :=
-  sorry
+  have h : (∀x : Prop, x = False ∧ True) ↔ True := 
+    (All.one_point_wrong False (fun _ ↦ True))
+  have h'' : ∀x : Prop, x = False ∧ True := Iff.mpr h True.intro
+  have h''' : True = False := (h'' True).left
+  show False from Eq.mp h''' True.intro
+
 
 /- 3.2 (**optional**). Prove that the following wrong formulation of the
 one-point rule for `∃` is inconsistent, using a structured proof. -/
@@ -108,8 +163,18 @@ one-point rule for `∃` is inconsistent, using a structured proof. -/
 axiom Exists.one_point_wrong {α : Type} (t : α) (P : α → Prop) :
   (∃x : α, x = t → P x) ↔ P t
 
+#check Exists.elim
+#check Exists.intro
+
 theorem Exists.proof_of_False :
   False :=
-  sorry
+  have h : (∃x : Prop, x = True → False) ↔ False := 
+    (Exists.one_point_wrong True (fun _ ↦ False))
+  show False from Iff.mp h (Exists.intro (¬ True) (
+    assume h'' : (¬ True) = True
+    show False from
+      by
+        simp at h''
+    ))
 
 end LoVe
