lean/LoVe/LoVe04_ForwardProofs_HomeworkSheet.lean
@@ -40,14 +40,27 @@ Hint: There is an easy way. -/
 
 theorem about_Impl_term :
   ∀a b : Prop, ¬ a ∨ b → a → b :=
-  sorry
+  fun _ _ h ha ↦ Or.elim h (fun hna ↦ False.elim (hna ha)) (·)
 
 /- 1.2 (2 points). Prove the same theorem again, this time by providing a
 structured proof, with `fix`, `assume`, and `show`. -/
 
 theorem about_Impl_struct :
   ∀a b : Prop, ¬ a ∨ b → a → b :=
-  sorry
+  fix a b : Prop
+  assume h : ¬ a ∨ b
+  assume ha : a
+  show b from 
+    Or.elim 
+    h 
+    (
+      assume hna : ¬ a
+      show b from False.elim (hna ha)
+    )
+    (
+      assume hb : b
+      show b from hb
+    )
 
 
 /- ## Question 2 (6 points): Connectives and Quantifiers
@@ -58,7 +71,39 @@ rules for `∀`, `∨`, and `↔`. -/
 
 theorem Or_comm_under_All {α : Type} (p q : α → Prop) :
   (∀x, p x ∨ q x) ↔ (∀x, q x ∨ p x) :=
-  sorry
+  show (∀x, p x ∨ q x) ↔ (∀x, q x ∨ p x) from
+    Iff.intro
+    (
+      assume h : ∀x, p x ∨ q x
+      fix x : α
+      show q x ∨ p x from
+        Or.elim 
+        (h x) 
+        (
+          assume h' : p x
+          show q x ∨ p x from Or.inr h'
+        )
+        (
+          assume h' : q x
+          show q x ∨ p x from Or.inl h'
+        )
+    )
+    (
+      assume h : ∀x, q x ∨ p x
+      fix x : α
+      show p x ∨ q x from
+        Or.elim
+        (h x)
+        (
+          assume h' : q x
+          show p x ∨ q x from Or.inr h'
+        )
+        (
+          assume h' : p x
+          show p x ∨ q x from Or.inl h'
+        )
+    )
+
 
 /- 2.2 (3 points). We have proved or stated three of the six possible
 implications between `ExcludedMiddle`, `Peirce`, and `DoubleNegation` in the
@@ -73,15 +118,18 @@ namespace BackwardProofs
 
 theorem Peirce_of_DN :
   DoubleNegation → Peirce :=
-  sorry
+  assume dn : DoubleNegation
+  show Peirce from Peirce_of_EM (SorryTheorems.EM_of_DN dn)
 
 theorem EM_of_Peirce :
   Peirce → ExcludedMiddle :=
-  sorry
+  assume p : Peirce
+  show ExcludedMiddle from SorryTheorems.EM_of_DN (DN_of_Peirce p)
 
 theorem dn_of_em :
   ExcludedMiddle → DoubleNegation :=
-  sorry
+  assume em : ExcludedMiddle
+  show DoubleNegation from DN_of_Peirce (Peirce_of_EM em)
 
 end BackwardProofs
 
