lean/LoVe/LoVe14_RationalAndRealNumbers_ExerciseSheet.lean
@@ -28,8 +28,13 @@ Hints:
 
 theorem Fraction.ext (a b : Fraction) (hnum : Fraction.num a = Fraction.num b)
     (hdenom : Fraction.denom a = Fraction.denom b) :
-  a = b :=
-  sorry
+  a = b := by
+  cases a
+  cases b
+  simp at *
+  apply And.intro
+  exact hnum
+  exact hdenom
 
 /- 1.2. Extending the `Fraction.Mul` instance from the lecture, declare
 `Fraction` as an instance of `Semigroup`.
@@ -43,8 +48,13 @@ Hint: Use the theorem `Fraction.ext` above, and possibly `Fraction.mul_num` and
 
 instance Fraction.Semigroup : Semigroup Fraction :=
   { Fraction.Mul with
-    mul_assoc :=
-      sorry
+    mul_assoc := by
+      intro a b c
+      apply Fraction.ext
+      . simp [Fraction.mul_num]
+        ac_rfl
+      . simp [Fraction.mul_denom]
+        ac_rfl
   }
 
 /- 1.3. Extending the `Rat.Mul` instance from the lecture, declare `Rat` as an
@@ -52,8 +62,13 @@ instance of `Semigroup`. -/
 
 instance Rat.Semigroup : Semigroup Rat :=
   { Rat.Mul with
-    mul_assoc :=
-      sorry
+    mul_assoc := by
+      intro a b c
+      induction a using Quotient.inductionOn
+      induction b using Quotient.inductionOn
+      induction c using Quotient.inductionOn
+      apply Quotient.sound
+      ac_rfl
   }
 
 end LoVe
